ulc: basics

Ttfp/Basic.lean
@@ -1,1 +1,68 @@
-def hello := "world"
+import Batteries.Data.RBMap.Basic
+
+-- 1.3.2: The set Λ of all λ-terms
+@[reducible] def Name := String
+
+inductive Λ where
+| var : Name → Λ
+| app : Λ → Λ → Λ
+| abs : Name → Λ → Λ
+deriving Repr, BEq, Ord
+
+namespace Λ
+
+-- 1.3.5: Multiset of subterms
+def Sub (t : Λ) : List Λ :=
+  match t with
+  | var _ => [t]
+  | app M N => t :: (Sub M ++ Sub N)
+  | abs _ M => t :: Sub M
+
+def Subterm (L M : Λ) : Prop := L ∈ Sub M
+
+-- instance : LawfulBEq Λ where
+--   eq_of_beq beq := rfl
+--   rfl := _
+-- instance (L : Λ) (M : Λ) : Decidable (Subterm L M) :=
+--   List.instDecidableMemListInstMembershipList L (Sub M)
+
+-- 1.3.6
+theorem Reflexivity (M : Λ) : Subterm M M := by
+  sorry
+  -- simp [Subterm, Sub]
+
+theorem Transitivity (L M N : Λ) : Subterm L M ∧ Subterm M N → Subterm L N := sorry
+
+-- 1.3.8: Proper subterm
+def ProperSubterm (L M : Λ) : Prop := Subterm L M ∧ L ≠ M
+
+-- 1.4.1: The set of free variables of a λ-term
+def FreeVariables : Λ → Batteries.RBSet Λ compare
+| t@(var _) => Batteries.RBSet.single t
+| app M N => FreeVariables M ∪ FreeVariables N
+| abs x M => FreeVariables M \ Batteries.RBSet.single (var x)
+
+-- 1.4.3: Closed λ-term; combinator; Λ⁰
+def Closed (M : Λ) : Prop := FreeVariables M = ∅
+
+-- 1.5.1: Renaming; Mˣ ʸ; =ₐ
+def rename (x y : Name) : Λ → Λ
+| t@(var z) => if z == x then var y else t
+| app M N => app (rename x y M) (rename x y N)
+| abs z M => abs (if z == x then y else z) (if z == x then M else rename x y M)
+
+def Renaming (M : Λ) (x y : Name) (N : Λ) : Prop := rename x y M = N
+
+-----
+
+def ex : Λ := abs "x" (app (var "x") (var "y"))
+
+#eval Sub ex
+-- #eval Subterm (var "x") ex
+-- #eval ProperSubterm (var "x") ex
+#eval FreeVariables ex
+#eval FreeVariables $ app (var "x") (abs "x" (app (var "x") (var "y")))
+-- #eval Closed $ abs "x" (var "x")
+#eval rename "x" "a" ex |> rename "x" "b"
+
+end Λ
