lakefile.lean
@@ -7,6 +7,8 @@ package «ttfp» where
 lean_lib «Ttfp» where
   -- add library configuration options here
 
+require batteries from git "https://github.com/leanprover-community/batteries" @ "main"
+
 @[default_target]
 lean_exe «ttfp» where
   root := `Main
